sepcomp/backend/Deadcodeproof_sepcomp.v
@@ -397,11 +397,11 @@ Let rm := romem_for_program prog.
 
 Lemma symbols_preserved:
   forall (s: ident), Genv.find_symbol tge s = Genv.find_symbol ge s.
-Proof (find_symbol_transf_partial' _ _ TRANSF).
+Proof (find_symbol_transf_partial_optionally _ _ TRANSF).
 
 Lemma varinfo_preserved:
   forall b, Genv.find_var_info tge b = Genv.find_var_info ge b.
-Proof (find_var_info_transf_partial' _ _ TRANSF).
+Proof (find_var_info_transf_partial_optionally _ _ TRANSF).
 
 Lemma functions_translated:
   forall (v: val) (f: RTL.fundef),
@@ -409,7 +409,7 @@ Lemma functions_translated:
   exists tf, Genv.find_funct tge v = Some tf /\ 
              match_fundef prog f tf.
 Proof.
-  intros. exploit (find_funct_transf_partial' _ _ TRANSF); eauto. simpl in *.
+  intros. exploit (find_funct_transf_partial_optionally _ _ TRANSF); eauto. simpl in *.
   intros [tf [Htf [[sprog [Hsprog Hf]]|Hf]]].
   eexists. split; eauto. econstructor. eauto.
   destruct f; monadInv Hf; auto.
@@ -424,7 +424,7 @@ Lemma function_ptr_translated:
   exists tf, Genv.find_funct_ptr tge b = Some tf /\ 
              match_fundef prog f tf.
 Proof.
-  intros. exploit (find_funct_ptr_transf_partial' _ _ TRANSF); eauto. simpl in *.
+  intros. exploit (find_funct_ptr_transf_partial_optionally _ _ TRANSF); eauto. simpl in *.
   intros [tf [Htf [[sprog [Hsprog Hf]]|Hf]]].
   eexists. split; eauto. econstructor. eauto.
   destruct f; monadInv Hf; auto.
@@ -1160,7 +1160,7 @@ Proof.
   exploit function_ptr_translated; eauto. intros (tf & A & B).
   exists (Callstate nil tf nil m0); split.
   econstructor; eauto.
-  exploit (init_mem_transf_partial' _ _ TRANSF); eauto.
+  exploit (init_mem_transf_partial_optionally _ _ TRANSF); eauto.
   replace (prog_main tprog) with (prog_main prog).
   rewrite symbols_preserved. eauto.
   inv TRANSF. auto.
